Complete preliminary coding of task5 in Coq

formal/coqimp/digsim5.v
@@ -12,7 +12,29 @@
 
  *)
 
+From RecordUpdate Require Import RecordUpdate.
+Module RecordSetNotations'.
+  Delimit Scope record_set with rs.
+  Open Scope rs.
+  (*
+    Note that the "set" function, after the proj argument, takes a function from 
+    the old value to the new value. "(constructor v)" will make such a function
+    that will ignore the old value and return v.
+  *)
+  Notation "x [[ proj  :=  v ]]" := (set proj (constructor v) x)
+                                    (at level 12, left associativity) : record_set.
+  Notation "x [[ proj  ::=  f ]]" := (set proj f x)
+                                     (at level 12, f at next level, left associativity) : record_set.
+End RecordSetNotations'.
+Import RecordSetNotations'.
+
 Require Import DigUty.float_text_io.
+Import FloatIO.
+Definition width := 15%nat.
+Definition fdigs := 6%nat.
+Definition f2s := float_to_string width fdigs.
+Definition fl2s := float_list_to_string width fdigs true.
+
 Require Import DigUty.Monad.
 
 From compcert Require Import Floats.
@@ -20,7 +42,9 @@ Import Float.
 From compcert Require Import Fappli_IEEE.
 From compcert Require Import Integers.
 Require Import Coq.Lists.List.
+
 Import ListNotations.
+
 Require Import BinNums.
 Require Import Coq.QArith.QArith_base.
 Require Import Strings.String.
@@ -28,8 +52,32 @@ Require Import Strings.Ascii.
 Require Import Coq.ZArith.Znat.
 Require Import Recdef.
 From compcert Require Import Maps.
-Import FloatIO.
-From RecordUpdate Require Import RecordUpdate.
+
+(*+ Float scope notations *)
+(* D for double float *)
+Bind Scope D_scope with float.
+Delimit Scope D_scope with D.
+
+Infix "+" := Float.add : D_scope.
+Notation "- x" := (Float.neg x) : D_scope.
+Infix "-" := Float.sub : D_scope.
+Infix "*" := Float.mul : D_scope.
+Infix "/" := Float.div : D_scope.
+Infix "?=" := Float.compare (at level 70, no associativity) : D_scope.
+
+Infix "=?" := (Float.cmp Ceq) (at level 70, no associativity) : D_scope.
+Infix "<=?" := (Float.cmp Cle) (at level 70, no associativity) : D_scope.
+Infix "<?" := (Float.cmp Clt) (at level 70, no associativity) : D_scope.
+Infix ">=?" := (Float.cmp Cge) (at level 70, no associativity) : D_scope.
+Infix ">?" := (Float.cmp Cgt) (at level 70, no associativity) : D_scope.
+Notation "0" := Float.zero : D_scope.
+
+(* Variant of strToFloat when we know the string is valid *)
+Definition strToFloat' (s: string) : float :=
+  match strToFloat s with
+  | Some x => x
+  | None => 0%D
+  end.
 
 (* Inductive type used to name state variables. *)
 Inductive StateVar : Set := 
@@ -52,6 +100,8 @@ Global Opaque state_var_eq.
 From compcert Require Import Decidableplus.
 
 Instance Decidable_eq_sv : forall (x y: StateVar), Decidable (eq x y) := Decidable_eq state_var_eq.
+
+
 
 (* For diagnostic purposes we want to map from the positive id for a
    StateVar to the StateVar. 
@@ -166,19 +216,53 @@ Compute svToStr svDT_PRINT.
 Definition FloatSvTree := SvTree.t float.
 Definition emptyFloatPTree := SvTree.empty float.
 
-Fixpoint UpdateFloatSvTree (valList: list (StateVar * string)) (intree: FloatSvTree) :=
+Fixpoint UpdateFloatSvTree (valList: list (StateVar * float)) (intree: FloatSvTree) :=
   match valList with
   | nil => intree
-  | cons (sv, str) vltail =>
-    let tree1 :=
-    match strToFloat str with
-    | Some val => SvTree.set sv val intree
-    | None => intree
-    end in
+  | cons (sv, fval) vltail =>
+    let tree1 := SvTree.set sv fval intree in
     UpdateFloatSvTree vltail tree1
   end.
 
-Definition initialValues :=
+(* Take state variable string pairs and convert to 
+   state variable float pairs, by converting each
+   string into a float. If the string cannot be converted,
+   then skip it.
+*)
+Fixpoint StringKeyValToFloatKeyVal (kvl: list (StateVar * string)) : list (StateVar * float) :=
+  match kvl with
+  | nil => nil
+  | cons (sv, str) tl =>
+    let tailkvs := StringKeyValToFloatKeyVal tl in
+    match strToFloat str with
+    | Some fval => (sv, fval) :: tailkvs
+    | None => tailkvs
+    end
+  end.
+
+Fixpoint PrintFloatKeyVals (kvl: list (StateVar * float)) :=
+  match kvl with
+  | nil => nil
+  | cons (sv, fval) tl =>
+    (sv, f2s fval) :: PrintFloatKeyVals tl
+  end.
+
+Definition driver_defaults_str :=
+  [
+            (svT,        "0.0");
+            (svT_STOP,   "0.0");
+            (svDT,       "0.005");
+            (svDT_MAX,   "0.005");
+            (svDT_MIN,   "0.005");
+            (svDT_PRINT, "0.01")
+  ].
+
+Definition driver_defaults :=
+  Eval compute in StringKeyValToFloatKeyVal driver_defaults_str.
+
+Compute PrintFloatKeyVals driver_defaults.
+
+Definition model_default_values_str :=
   [
     (svT,             "0.0");
     (svX,             "10.0");
@@ -193,18 +277,27 @@ Definition initialValues :=
     (svDT_PRINT,      "0.01")
   ].
 
-Definition state0 := Eval compute in UpdateFloatSvTree initialValues emptyFloatPTree.
+Definition model_default_values :=
+  Eval compute in StringKeyValToFloatKeyVal model_default_values_str.
+
+Compute PrintFloatKeyVals model_default_values.
+
+Definition state0 := Eval compute in
+      let driverState := UpdateFloatSvTree driver_defaults emptyFloatPTree in
+      UpdateFloatSvTree model_default_values driverState.
+
 
 Definition svToFloat0 (sv: StateVar) := SvTree.get sv state0.
 
 Definition svToFloatStr0 (sv: StateVar) :=
   match svToFloat0 sv with
-  | Some x => float_to_string 8 4 x
+  | Some x => f2s x
   | None => "None"
   end.
 
 Compute svToFloatStr0 svGRAVITY.
 
+(* Takes a long time.
 Lemma state0Complete:
   forall sv: StateVar, exists f: float,
       SvTree.get sv state0 = Some f.
@@ -212,62 +305,443 @@ Proof.
   intros.
   destruct sv;compute; eexists; f_equal.
 Qed.
+ *)
+
+(* Since we have proven that state is complete, we can define a
+   function that always returns a float, using a default
+   in the impossible case.
+ *)
+Definition svGetFloat (sv: StateVar) (tree : FloatSvTree) :=
+  match SvTree.get sv tree with
+  | Some x => x
+  | None => 0%D
+  end.
+
+Compute PTree.elements state0.
+
+
+(* Give StateVar given its positive id, or if not a valid id,
+   an arbitrary StateVar
+*)
+Definition posToStateVar' (pos: positive) :=
+  match posToStateVar pos with
+  | Some x => x
+  | None => svT
+  end.
+
+Fixpoint PrintFloatStateElements (elist: list (positive * float)) : list (StateVar * string) :=
+  match elist with
+  | nil => nil
+  | cons (pos, fval) tl =>
+    (posToStateVar' pos, f2s fval) :: PrintFloatStateElements tl
+  end.
+
+Definition PrintFloatState (state: FloatSvTree) :=
+  PrintFloatStateElements (PTree.elements state).
+
+Compute PrintFloatState state0.
 
 (*
-Compute SvTree.get svXD (SvTree.set svXD Float.zero emptyFloatPTree).
+Compute float_to_string 8 4 (svGetFloat svGRAVITY state0).
+Compute SvTree.get svXD (SvTree.set svXD 0%D emptyFloatPTree).
 *)
 
 Definition modelOutputs : list StateVar := [svT; svX; svXD].
 Print modelOutputs.
 
+Record Flags :=
+  mkFlags
+    {
+      stop_simulation : bool; (* Stop the simulation, t > tStop, *)
+      end_of_run : bool;      (* Terminate early, user event logic. *)
+      evaluate_xd : bool     (* Flag to determine of xd needs to reevaluated. *)
+    }.
 
+Instance etaFlags  : Settable _ := 
+  mkSettable (constructor mkFlags
+                          <*> stop_simulation
+                          <*> end_of_run
+                          <*> evaluate_xd
+             )%set.
 
-Definition ident := term.
-    
+Inductive EventFuncId :=
+| efiStop
+| efiAppendSolution
+| efiTerminateSim
+| efiFlip_Xd_At_Bounce
+.
 
-Definition _time: ident := 1.
+Record Event :=
+  mkEvent
+    {
+      key : string;
+      time : float;
+      func : EventFuncId
+    }.
 
+Instance etaEvent : Settable Event := 
+  mkSettable (constructor mkEvent
+                          <*> key
+                          <*> time
+                          <*> func
+             )%set.
 
-(** DigSim - Mass Spring Damper
+Record Sim :=
+  mkSim
+    {
+      vars : FloatSvTree;              (* Simulation variables and constants. *)
+      solkeys : list StateVar;         (* Keys of fields in Solution. *)
+      solution : list (list string);   (* Simulation detail results. *)
+      sim_events : list Event;   (* User events. *)
+      log : list string;               (* Text logging for debugging or information. *)
+      flags : Flags                    (* control flags *)
+    }.
+
+Instance etaSim  : Settable _ := 
+  mkSettable (constructor mkSim
+                          <*> vars
+                          <*> solkeys
+                          <*> solution
+                          <*> sim_events
+                          <*> log
+                          <*> flags
+             )%set.
+
+Definition default_flags :=
+  {|
+    stop_simulation := false;
+    end_of_run := false;
+    evaluate_xd := false;
+  |}.
+
+(* Return value is a pair of the updated sim, and an optional float which,
+   if present, is the new time at which the event should be scheduled.
+   The caller must do this.
  *)
-Definition time0               := Z_to_float 0                    . (* 0.0          simulation time [sec]                      *)
-Definition x_ic                := Z_to_float 0                    . (* 0.0          initial position of suspended mass [m]     *)
-Definition xd_ic               := Z_to_float 0                    . (* 0.0          initial velocity of suspended mass [m/sec] *)
-Definition mass                := Z_to_float 1                    . (* 1.0    1#1   mass suspended from spring [kg]            *)
-Definition tstop               := fraction_to_float  25  1        . (* 2.5    2#5   simulation stop time [sec]                 *)
-Definition dt                  := fraction_to_float   1  2        . (* 0.01   1#100 simulation time step [sec]                 *)
-Definition damping_coefficient := fraction_to_float 888  2        . (* 8.88 222#25  damping force per velocity [n/m/s]         *)
-Definition gravity             := fraction_to_float 988  2        . (* 9.88 247#25  acceleration due to gravity [m/sec**2]     *)
-Definition spring_coefficient  := fraction_to_float 3947 2        . (* 39.47 3947#100 restoring force per position [n/m]       *)
+Open Scope D_scope.
 
-Open Scope Z.
+Definition t_ge_tstop_event_func (this: Event) (sim: Sim) : (Sim * option float) :=
+  let vars := sim.(vars) in
+  let t := svGetFloat svT vars in
+  let t_stop := svGetFloat svT_STOP vars in
+  let stop_sim := t >=? t_stop in
+  let new_flags := sim.(flags)[[stop_simulation := stop_sim]] in
+  (sim[[flags := new_flags]], None).
 
-Definition xdd x xd : float :=
-  sub ( div (neg (add (mul spring_coefficient x)  (mul damping_coefficient xd)) ) mass) gravity.
+Fixpoint make_solution_row_helper (vars: FloatSvTree) (keys: list StateVar) : list string :=
+  match keys with
+  | nil => nil
+  | cons key others =>
+    let fval := svGetFloat key vars in
+    let sval := f2s fval in
+    sval :: make_solution_row_helper vars others
+  end.
 
-Definition step (t x xd : float) : (float * float * float) :=
-  let xdd' := xdd x xd             in
-  let x'   := add x  (mul xd   dt) in
-  let xd'  := add xd (mul xdd' dt) in
-  let t'   := add t dt             in
-  (t', x', xd').
+Definition make_solution_row (sim: Sim) :=
+  let row := make_solution_row_helper sim.(vars) sim.(solkeys) in
+  sim[[solution ::= (fun old => row :: old)]].
 
-Fixpoint advance (fuel : nat) (t x xd : float) : list (list float) :=
-match fuel with
-|  O   => nil
-|  S n =>
-   let '(t', x', xd') := (step t x xd) in
-   (t' :: x' :: xd' :: nil) :: (advance n t' x' xd')
-end.
+Definition append_solution_event_func (this: Event) (sim: Sim) : (Sim * option float) :=
+  let sim1 := make_solution_row sim in
+  let vars := sim1.(vars) in
+  let dt_print := svGetFloat svDT_PRINT vars in
+  let t := svGetFloat svT vars in
+  let new_t := t + dt_print in
+  (sim1, Some new_t).
 
-Definition width := 15%nat.
-Definition fdigs := 6%nat.
-Definition f2s := float_to_string width fdigs.
-Definition fl2s := float_list_to_string width fdigs true.
+Definition terminate_sim_event_func (this: Event) (sim: Sim) : (Sim * option float) :=
+  (sim, None).
 
-Definition digsim : string := nl ++ (fl2s (time0 :: x_ic :: xd_ic :: nil)) ++
-                        (concat "" (map fl2s (advance 250 time0 x_ic xd_ic))) ++ nl.
+Definition driver_default_events :=
+  [
+    {| key := "t_ge_tstop_event"; time := 0%D; func := efiStop|};
+    {| key := "append_log_event"; time := 0%D; func := efiAppendSolution|};
+    {| key := "terminate_sim_event"; time := 0%D; func := efiTerminateSim|}
+  ].
 
-Set Printing Depth 500.
-Set Printing Width 0.
-Compute digsim.
+Definition default_sim :=
+  {|
+    vars := state0;
+    solkeys := modelOutputs;
+    solution := nil;
+    sim_events := driver_default_events;
+    log := nil;
+    flags := default_flags;
+  |}.
+
+Definition F99 := Eval compute in strToFloat' "99.0".
+
+Definition bounceEvent :=
+  {| key := "flip_xd_at_bounce_event";
+     time := F99;
+     func := efiFlip_Xd_At_Bounce;
+  |}.
+
+Definition init_sim (sim: Sim) :=
+  sim[[sim_events ::= (fun evs => bounceEvent :: evs)]].
+
+Definition set_vars (sim: Sim) (vars' : FloatSvTree) :=
+  sim[[vars := vars']].
+
+Definition flip_xd_at_bounce_event_func (this: Event) (sim: Sim) : (Sim * option float) :=
+  let vars := sim.(vars) in
+  let coeff_of_rest := svGetFloat svCOEFF_OF_REST vars in
+  let xd := svGetFloat svXD vars in
+  let new_xd := - (coeff_of_rest * xd) in
+  let vars' := SvTree.set svXD new_xd vars in
+  let new_flags := sim.(flags)[[evaluate_xd := true]] in
+  let sim' := set_vars sim vars' in
+  let sim'' := sim'[[flags := new_flags]] in
+  (sim', Some F99).
+
+Definition handle_event (this: Event) (sim: Sim) : (Sim * option float) :=
+  match this.(func) with
+  | efiStop => t_ge_tstop_event_func this sim
+  | efiAppendSolution => append_solution_event_func this sim
+  | efiTerminateSim => terminate_sim_event_func this sim
+  | efiFlip_Xd_At_Bounce => flip_xd_at_bounce_event_func this sim
+  end.
+
+Definition set_var (key: StateVar) (val: float) (sim: Sim) :=
+  sim[[vars := SvTree.set key val sim.(vars)]].
+
+Definition F0p5 := Eval compute in strToFloat' "0.5".
+Definition Ftwo := Eval compute in strToFloat' "2.0".
+
+(* pi matching Haskell Prelude Double *)
+Definition PI := Eval compute in strToFloat' "3.141592653589793238".
+
+(* small floating point constant *)
+Definition SMALL := Eval compute in strToFloat' "0.000001".
+
+(* comparison floating point constant *)
+Definition EPSILON := Eval compute in strToFloat' "0.0000000001".
+(* Compute float_to_string 0 19 PI. *)
+
+Definition efi_eqb (fi1 fi2 : EventFuncId) : bool :=
+  match fi1, fi2 with
+  | efiStop, efiStop => true
+  | efiAppendSolution, efiAppendSolution => true
+  | efiTerminateSim, efiTerminateSim => true
+  | efiFlip_Xd_At_Bounce, efiFlip_Xd_At_Bounce => true
+  | _, _ => false
+  end.
+
+(* Update a list of events by changing the scheduled time for the 
+   one with the specified function id.
+*)
+Fixpoint schedule_event (evs: list Event) (efi: EventFuncId) (new_time: float) :=
+  match evs with
+  | nil => nil
+  | cons ev evtl =>
+    let ev' :=
+        if efi_eqb ev.(func) efi then
+          ev[[time := new_time]]
+        else
+          ev
+    in
+    ev' :: schedule_event evtl efi new_time
+  end.
+
+Definition sqrt (arg: float) : float :=
+  Fappli_IEEE_bits.b64_sqrt mode_NE arg.
+(*
+Definition F9 := Eval compute in strToFloat' "9.0".
+Definition sqrt9 := Eval compute in sqrt F9.
+Compute f2s sqrt9.
+ *)
+
+Definition F1 := Eval compute in strToFloat' "1.0".
+
+Definition differential_equations (sim: Sim) : Sim :=
+  let vars := sim.(vars) in
+  let t := svGetFloat svT vars in
+  let x := svGetFloat svX vars in
+  let xd := svGetFloat svXD vars in
+  let dt_min := svGetFloat svDT_MIN vars in
+  let dt_max := svGetFloat svDT_MAX vars in
+  let gravity := svGetFloat svGRAVITY vars in
+  let t_stop := svGetFloat svT_STOP vars in
+
+  let xdd := -gravity in
+  let sim1 := set_var svXDD xdd sim in
+  let est_max := x + xd * dt_max + F0p5 * xdd * dt_max * dt_max in
+  let dt_impact := t_stop + F1 in
+  let dt_impact2 :=
+      if (est_max <=? 0%D) then
+        let est_min := x + xd * dt_min + F0p5 * xdd * dt_min * dt_min in
+        if (est_min <=? 0%D) then
+            0%D
+        else
+            let dt_impact3 := (-xd - sqrt(xd * xd - Ftwo * x * xdd)) / (Ftwo * x) in
+            if (dt_min - dt_impact3 >? EPSILON) then
+              (-xd + sqrt(xd * xd - Ftwo * x * xdd)) / (Ftwo * x)
+            else
+              dt_impact3
+      else
+        dt_impact in
+  let impact_time := t + dt_impact2 in
+  let events' := schedule_event sim1.(sim_events) efiFlip_Xd_At_Bounce impact_time in
+  let sim2 := sim1[[sim_events := events']] in
+  sim2.
+
+Definition round (f: float) : Z :=
+  let maybe_vlong := to_long f in
+  let v64 :=
+      match maybe_vlong with
+      | Some x => x
+      | None => Int64.zero
+      end in
+  Int64.intval v64.
+
+Definition TenTo6 := Eval compute in strToFloat' "1.e6".
+
+Definition process_one_event (ev: Event) (sim: Sim) :=
+  let vars := sim.(vars) in
+  let t := svGetFloat svT vars in
+  let dt_min := svGetFloat svDT_MIN vars in
+  let dt_max := svGetFloat svDT_MAX vars in
+  let et := ev.(time) in
+  let etdelta := round ((et - t) * TenTo6) in
+  let minrnd := round (dt_min * TenTo6) in
+  let (ev', sim') :=
+      if (etdelta <? minrnd)%Z then
+        let (sim2, new_time_opt) := handle_event ev sim in
+        match new_time_opt with
+        | Some new_time => (ev[[time := new_time]], sim2)
+        | None => (ev, sim2)
+        end
+      else
+        (ev, sim)
+  in
+  (ev', sim').
+
+Fixpoint process_events_helper (evs: list Event) (sim: Sim) :=
+  match evs with
+  | nil => (nil, sim)
+  | cons ev evtl =>
+    let (ev', sim') := process_one_event ev sim in
+    let (evs', sim'') := process_events_helper evtl sim' in
+    (ev' :: evs', sim'')
+  end.
+
+Fixpoint min_event_time (evs: list Event) (min_so_far: float) : float :=
+  match evs with
+  | nil => min_so_far
+  | cons ev evtl =>
+    let et := ev.(time) in
+    let new_min :=
+        if (et >? 0%D) && (et <? min_so_far) then
+          et
+        else
+          min_so_far
+    in
+    min_event_time evtl new_min
+  end.
+
+  
+Definition process_events (sim: Sim) : Sim :=
+  let vars0 := sim.(vars) in
+  let events := sim.(sim_events) in
+  match events with
+  | nil => set_var svDT (svGetFloat svDT_MAX vars0) sim
+  | cons x x0 =>
+    let t := svGetFloat svT vars0 in
+    let dt_max := svGetFloat svDT_MAX vars0 in
+    let (evs', sim') := process_events_helper events sim in
+    let vars' := sim'.(vars) in
+    let min_time0 := svGetFloat svT_STOP vars' in
+    let min_time := min_event_time evs' min_time0 in
+    let time_to_next_event := min_time - t in
+    let new_dt :=
+        if (time_to_next_event >? 0%D) && ((dt_max - time_to_next_event) >? EPSILON) then
+          time_to_next_event
+        else
+          dt_max
+    in
+    let sim3 := set_var svDT new_dt sim' in
+    let sim4 := sim3[[sim_events := evs']] in
+    sim4
+  end.
+
+Fixpoint advance_states (pairs: list (StateVar * StateVar)) (dt: float) (sim: Sim) : Sim :=
+  match pairs with
+  | nil => sim
+  | cons (sv, svd) pairstl =>
+    let vars0 := sim.(vars) in
+    let el := svGetFloat sv vars0 in
+    let eld := svGetFloat svd vars0 in
+    let el' := el + eld * dt in
+    let sim' := set_var sv el' sim in
+    let sim'' := advance_states pairstl dt sim' in
+    sim''
+  end.
+
+Definition advance_model (sim: Sim) : Sim :=
+  let vars0 := sim.(vars) in
+  let dt := svGetFloat svDT vars0 in
+  let pairs := [(svX, svXD); (svXD, svXDD) ] in
+  let sim' := advance_states pairs dt sim in
+  let vars' := sim'.(vars) in
+  let t := svGetFloat svT vars' in
+  let new_t := (Z_to_float (round(t * TenTo6)))/TenTo6 in
+  let sim'' := set_var svT new_t sim' in
+  sim''.
+
+Definition oneStep (sim: Sim) : Sim :=
+  let sim1 := differential_equations sim in
+  let sim2 := process_events sim1 in
+  let sim3 :=
+      if sim2.(flags).(evaluate_xd) then
+        let sim4 := differential_equations sim2 in
+        let flags4 := sim4.(flags) in
+        let flags4' := flags4[[evaluate_xd := false]] in
+        sim4[[flags := flags4']]
+      else
+        sim2 in
+  let sim5 := advance_model sim3 in
+  sim5.
+
+Require Import Zwf.
+From compcert Require Import Coqlib.
+
+Function run_sim_loop (steps: Z) (sim: Sim) { wf (Zwf 0%Z) steps } :=
+  if zle 0%Z steps
+  then
+    let f := sim.(flags) in
+    if f.(end_of_run) || f.(stop_simulation)
+    then sim
+    else run_sim_loop (steps - 1) (oneStep sim)
+  else sim.
+Proof.
+  intros; red; omega.
+  apply Zwf_well_founded.
+Qed.
+
+(*
+Definition binary64 := binary_float 53 1024.
+*)
+
+Definition ZofFloat (f: float) :=
+  match Fappli_IEEE_extra.ZofB 53 1024 f with
+  | Some z => z
+  | None => 0
+  end.
+
+Definition run_sim (sim: Sim) :=
+  let vars := sim.(vars) in
+  let dtmin := svGetFloat svDT_MIN vars in
+  let tstop := svGetFloat svT_STOP vars in
+  let max_steps_float := (tstop / dtmin)%D in
+  let steps := ZofFloat max_steps_float in
+  run_sim_loop steps sim.
+
+Definition main :=
+  let sim1 := default_sim in
+  let sim2 := init_sim sim1 in
+  let sim3 := set_var svCOEFF_OF_REST (strToFloat' "0.88") sim2 in
+  let sim4 := set_var svGRAVITY (strToFloat' "9.88") sim3 in
+  let sim5 := run_sim sim4 in
+  sim5.
+
+Compute main.
